Do AST generation for expressions I can parse (except infixes)

compiler/parsing/selftest.sml
@@ -5,7 +5,9 @@ val errcount = ref 0
 val _ = diemode := Remember errcount
 
 val _ = computeLib.add_funs [lexer_funTheory.get_token_def,
-                             listTheory.LIST_REL_def]
+                             listTheory.LIST_REL_def,
+                             ASCIInumbersTheory.s2n_compute,
+                             numposrepTheory.l2n_def]
 
 val gencst = “λn s. ispeg_exec purePEG (nt (INL n) I lrOK) (lexer_fun s)
                              lpTOP [] NONE [] done failed”
@@ -17,8 +19,9 @@ val fullparse =
                Result (Success [] [pt] _ _) => f pt
              | _ => (NONE : α option)”;
 
+fun KNL s = String.translate (fn #"\n" => "\\n" | c => str c) s
 fun fptest (nt, s, cf, exp) =
-    (tprint ("Parsing (" ^ term_to_string nt ^ ") \"" ^ s ^ "\"");
+    (tprint ("Parsing (" ^ term_to_string nt ^ ") \"" ^ KNL s ^ "\"");
      require_msg (check_result (aconv exp)) term_to_string
                  (rand o rhs o concl o EVAL)
                  (list_mk_icomb(fullparse,
@@ -30,6 +33,14 @@ val _ = app fptest [
   (“nTy”, "a -> B", “astType nTy”, “funTy (tyVar "a") (tyOp "B" [])”),
   (“nTy”, "(Tree a, B)", “astType nTy”, “tyTup [tyOp "Tree" [tyVar "a"];
                                                 tyOp "B" []]”),
-  (“nTy”, "[Int -> ()]", “astType nTy”, “listTy (funTy intTy $ tyTup [])”)
+  (“nTy”, "[Int -> ()]", “astType nTy”, “listTy (funTy intTy $ tyTup [])”),
+  (“nExp”, "f 2 x", “astExp nExp”,
+   “expApp (expApp (expVar "f") (expLit $ litInt 2)) (expVar "x")”),
+  (“nExp”, "\\x y -> y x", “astExp nExp”,
+   “expAbs (patVar "x")
+     (expAbs (patVar "y") (expApp (expVar "y") (expVar "x")))”),
+  (“nExp”, " if p x \nthen 1 else 2", “astExp nExp”,
+   “expIf (expApp (expVar "p") (expVar "x")) (expLit (litInt 1))
+          (expLit (litInt 2)) ”)
 ]
 
