compiler/parsing/cst_to_astScript.sml
@@ -24,6 +24,35 @@ Definition mkFunTy_def:
   mkFunTy (ty::rest) = tyOp "Fun" [ty; mkFunTy rest]
 End
 
+Definition grab_def:
+  grab f [] = SOME ([], []) ∧
+  grab f (h::t) =
+  do
+    v <- f h;
+    (vs, tail) <- grab f t;
+    SOME (v::vs, tail)
+  od ++ SOME([], h::t)
+End
+
+Theorem grab_EQ_SOME_APPEND:
+  ∀xs res xs'. grab f xs = SOME (res, xs') ⇒
+               ∃px. xs = px ++ xs'
+Proof
+  Induct_on ‘xs’ >>
+  simp[grab_def, miscTheory.option_eq_some, DISJ_IMP_THM, PULL_EXISTS,
+       pairTheory.FORALL_PROD] >> rpt strip_tac >>
+  first_x_assum $ drule_then strip_assume_tac >> rw[]
+QED
+
+Theorem grab_cong[defncong]:
+  ∀l1 l2 f1 f2. l1 = l2 ∧ (∀e. MEM e l2 ⇒ f1 e = f2 e) ⇒
+                grab f1 l1 = grab f2 l2
+Proof
+  simp[] >> Induct >>
+  simp[grab_def, DISJ_IMP_THM, FORALL_AND_THM, miscTheory.option_eq_some]>>
+  rpt strip_tac >> first_x_assum drule >> simp[]
+QED
+
 
 Definition astType_def:
   astType nt (Lf _) = NONE ∧
@@ -109,5 +138,109 @@ Termination
                            | INR (INR pts) => ptlsize pts)’ >> rw[]
 End
 
+
+Definition astLit_def:
+  astLit (Lf _) = NONE ∧
+  astLit (Nd nt args) =
+  if FST nt ≠ INL nLit then NONE
+  else
+    case args of
+      [] => NONE
+    | [pt] => lift litInt $ destIntT ' (destTOK ' (destLf pt))
+    | _ => NONE
+End
+
+Theorem SUM_MAP_EL_lemma:
+  ∀xs i. i < LENGTH xs ⇒ f (EL i xs) ≤ SUM (MAP f xs)
+Proof
+  Induct >> simp[] >> Cases_on ‘i’ >> simp[] >> rpt strip_tac >>
+  first_x_assum drule >> simp[]
+QED
+
+Definition astPat_def:
+  astPat _ (Lf _) = NONE ∧
+  (astPat nt1 (Nd nt2 args) =
+   if INL nt1 ≠ FST nt2 then NONE
+   else if nt1 = nAPat then
+     case args of
+       [pt] => do
+                vnm <- destAlphaT ' (destTOK ' (destLf pt));
+                SOME $ patVar vnm
+              od ++ (lift patLit $ astLit pt)
+     | _ => NONE
+   else NONE)
+End
+
+
+Definition astExp_def:
+  astExp _ (Lf _) = NONE ∧
+  (astExp nt1 (Nd nt2 args) =
+   if INL nt1 ≠ FST nt2 then NONE
+   else if nt1 = nAExp then
+     case args of
+       [pt] =>
+         do
+           vnm <- destAlphaT ' (destTOK ' (destLf pt)) ;
+           SOME $ expVar vnm
+         od ++ (lift expLit $ astLit pt)
+     | [lp;ept;rp] =>
+         do
+           assert (tokcheck lp LparT ∧ tokcheck rp RparT);
+           astExp nExp ept;
+         od
+     | _ => NONE
+   else if nt1 = nExp then
+     case args of
+       [pt] => astExp nIExp pt
+     | pt1::rest =>
+         do
+           assert (tokcheck pt1 IfT ∧ LENGTH rest = 5 ∧
+                   LIST_REL (λP pt. P pt) [K T; flip tokcheck ThenT; K T;
+                                           flip tokcheck ElseT; K T]
+                            rest);
+           gd_e <- astExp nExp ' (oEL 0 rest);
+           then_e <- astExp nExp ' (oEL 2 rest);
+           else_e <- astExp nExp ' (oEL 4 rest);
+           SOME $ expIf gd_e then_e else_e;
+         od ++
+         do
+           assert (tokcheck pt1 (SymbolT "\\"));
+           (pats,tail) <- grab (astPat nAPat) rest;
+           assert (LIST_REL (λP pt. P pt) [flip tokcheck ArrowT; K T] tail);
+           body_e <- astExp nExp ' (oEL 1 tail);
+           SOME $ FOLDR expAbs body_e pats
+         od
+     | _ => NONE
+   else if nt1 = nIExp then
+     case args of
+       [pt] => astExp nFExp pt
+     | _ => NONE
+   else if nt1 = nFExp then
+     case args of
+       [] => NONE
+     | fpt :: rest =>
+         do
+           f_e <- astExp nAExp fpt;
+           (aes, tail) <- grab (astExp nAExp) rest;
+           assert (NULL tail);
+           SOME $ FOLDL expApp f_e aes
+         od
+   else
+     NONE)
+Termination
+  WF_REL_TAC ‘measure (ptree_size o SND)’ >> simp[miscTheory.LLOOKUP_EQ_EL] >>
+  rpt strip_tac >~
+  [‘MEM x xs’, ‘ptree_size x < _’, ‘MAP ptree_size xs’]
+  >- (‘ptree_size x ≤ SUM (MAP ptree_size xs)’ suffices_by simp[] >>
+      qpat_x_assum ‘MEM _ _’ mp_tac >> Induct_on ‘xs’ >> simp[DISJ_IMP_THM] >>
+      rpt strip_tac >> gs[]) >>
+  TRY (drule_then strip_assume_tac grab_EQ_SOME_APPEND >>
+       pop_assum (assume_tac o Q.AP_TERM ‘SUM o MAP ptree_size’) >>
+       gs[listTheory.SUM_APPEND]) >>
+  qmatch_goalsub_abbrev_tac ‘ptree_size (EL i ptl)’ >>
+  ‘ptree_size (EL i ptl) ≤ SUM (MAP ptree_size ptl)’
+    suffices_by simp[Abbr‘i’] >>
+  simp[Abbr‘i’, Abbr‘ptl’, SUM_MAP_EL_lemma]
+End
 
 val _ = export_theory();
